Replace panicking integer ops by custom typeclasses (+?, -?, etc.)

src/pure/PrintPure.ml
@@ -888,7 +888,7 @@ let cast_kind_to_string (env : fmt_env) (kind : cast_kind) : string =
 let unop_to_string (env : fmt_env) (unop : unop) : string =
   match unop with
   | Not _ -> "¬"
-  | Neg _ -> "-"
+  | Neg _ -> "-?"
   | Cast kind -> cast_kind_to_string env kind
   | ArrayToSlice -> "array_to_slice"
 
