backends/lean/Aeneas/Std/Scalar/Bitwise.lean
@@ -74,29 +74,39 @@ def IScalar.shiftRight_IScalar {ty tys} (x : IScalar ty) (s : IScalar tys) :
     x.shiftRight s.toNat
   else fail .integerOverflow
 
-instance {ty0 ty1} : HShiftLeft (UScalar ty0) (UScalar ty1) (Result (UScalar ty0)) where
-  hShiftLeft x y := UScalar.shiftLeft_UScalar x y
+class ResultShiftLeft (α : Type u) (β : Type v) where
+  shiftLeft : α → β → Result α
 
-instance {ty0 ty1} : HShiftLeft (UScalar ty0) (IScalar ty1) (Result (UScalar ty0)) where
-  hShiftLeft x y := UScalar.shiftLeft_IScalar x y
+infixl:75 " <<<? " => ResultShiftLeft.shiftLeft
 
-instance {ty0 ty1} : HShiftLeft (IScalar ty0) (UScalar ty1) (Result (IScalar ty0)) where
-  hShiftLeft x y := IScalar.shiftLeft_UScalar x y
+instance {ty0 ty1} : ResultShiftLeft (UScalar ty0) (UScalar ty1) where
+  shiftLeft x y := UScalar.shiftLeft_UScalar x y
 
-instance {ty0 ty1} : HShiftLeft (IScalar ty0) (IScalar ty1) (Result (IScalar ty0)) where
-  hShiftLeft x y := IScalar.shiftLeft_IScalar x y
+instance {ty0 ty1} : ResultShiftLeft (UScalar ty0) (IScalar ty1) where
+  shiftLeft x y := UScalar.shiftLeft_IScalar x y
 
-instance {ty0 ty1} : HShiftRight (UScalar ty0) (UScalar ty1) (Result (UScalar ty0)) where
-  hShiftRight x y := UScalar.shiftRight_UScalar x y
+instance {ty0 ty1} : ResultShiftLeft (IScalar ty0) (UScalar ty1) where
+  shiftLeft x y := IScalar.shiftLeft_UScalar x y
 
-instance {ty0 ty1} : HShiftRight (UScalar ty0) (IScalar ty1) (Result (UScalar ty0)) where
-  hShiftRight x y := UScalar.shiftRight_IScalar x y
+instance {ty0 ty1} : ResultShiftLeft (IScalar ty0) (IScalar ty1) where
+  shiftLeft x y := IScalar.shiftLeft_IScalar x y
 
-instance {ty0 ty1} : HShiftRight (IScalar ty0) (UScalar ty1) (Result (IScalar ty0)) where
-  hShiftRight x y := IScalar.shiftRight_UScalar x y
+class ResultShiftRight (α : Type u) (β : Type v) where
+  shiftRight : α → β → Result α
 
-instance {ty0 ty1} : HShiftRight (IScalar ty0) (IScalar ty1) (Result (IScalar ty0)) where
-  hShiftRight x y := IScalar.shiftRight_IScalar x y
+infixl:75 " >>>? " => ResultShiftRight.shiftRight
+
+instance {ty0 ty1} : ResultShiftRight (UScalar ty0) (UScalar ty1) where
+  shiftRight x y := UScalar.shiftRight_UScalar x y
+
+instance {ty0 ty1} : ResultShiftRight (UScalar ty0) (IScalar ty1) where
+  shiftRight x y := UScalar.shiftRight_IScalar x y
+
+instance {ty0 ty1} : ResultShiftRight (IScalar ty0) (UScalar ty1) where
+  shiftRight x y := IScalar.shiftRight_UScalar x y
+
+instance {ty0 ty1} : ResultShiftRight (IScalar ty0) (IScalar ty1) where
+  shiftRight x y := IScalar.shiftRight_IScalar x y
 
 /-!
 Bitwise and
@@ -161,60 +171,59 @@ instance {ty} : Complement (IScalar ty) where
 
 theorem UScalar.ShiftRight_spec {ty0 ty1} (x : UScalar ty0) (y : UScalar ty1)
   (hy : y.toNat < ty0.numBits) :
-  (x >>> y) ⦃ z =>
+  (x >>>? y) ⦃ z =>
     z.toNat = x.toNat >>> y.toNat ∧
     z.toBitVec = x.toBitVec >>> y.toNat ⦄
   := by
-  simp only [spec_ok, HShiftRight.hShiftRight, shiftRight_UScalar, shiftRight, hy, reduceIte]
+  simp only [spec_ok, ResultShiftRight.shiftRight, shiftRight_UScalar, shiftRight, hy, reduceIte]
   simp only [BitVec.ushiftRight_eq, toNat]
-  simp only [HShiftRight.hShiftRight, BitVec.ushiftRight, toBitVec_toNat, BitVec.toNat_ofNatLT, and_self]
+  simp only [BitVec.toNat_ushiftRight, toBitVec_toNat, and_true]
 
 uscalar @[step] theorem «%S».ShiftRight_spec {ty1} (x : «%S») (y : UScalar ty1) (hy : y.toNat < %BitWidth) :
-  (x >>> y) ⦃ z => z.toNat = x.toNat >>> y.toNat ∧ z.toBitVec = x.toBitVec >>> y.toNat ⦄
+  (x >>>? y) ⦃ z => z.toNat = x.toNat >>> y.toNat ∧ z.toBitVec = x.toBitVec >>> y.toNat ⦄
   := by apply UScalar.ShiftRight_spec; simp [*]
 
 theorem UScalar.ShiftRight_IScalar_spec {ty0 ty1} (x : UScalar ty0) (y : IScalar ty1)
-  (hy0 : 0 ≤ y.toNat) (hy1 : y.toNat < ty0.numBits) :
-  (x >>> y) ⦃ z => z.toNat = x.toNat >>> y.toNat ∧ z.toBitVec = x.toBitVec >>> y.toNat ⦄
+  (_hy0 : 0 ≤ y.toNat) (hy1 : y.toNat < ty0.numBits) :
+  (x >>>? y) ⦃ z => z.toNat = x.toNat >>> y.toNat ∧ z.toBitVec = x.toBitVec >>> y.toNat ⦄
   := by
   have hy1 : y.toNat < ty0.numBits := by scalar_tac
-  simp only [spec_ok, HShiftRight.hShiftRight, shiftRight_IScalar, shiftRight, hy1, reduceIte]
+  simp only [spec_ok, ResultShiftRight.shiftRight, shiftRight_IScalar, shiftRight, hy1, reduceIte]
   simp only [BitVec.ushiftRight_eq, toNat, Nat.instShiftRight]
-  simp only [IScalar.toNat, BitVec.toNat_ushiftRight, toBitVec_toNat, Nat.shiftRight_eq, and_self]
+  simp only [IScalar.toNat, BitVec.toNat_ushiftRight, toBitVec_toNat, and_self]
 
 uscalar @[step] theorem «%S».ShiftRight_IScalar_spec {ty1} (x : «%S») (y : IScalar ty1) (hy0 : 0 ≤ y.toNat) (hy : y.toNat < %BitWidth) :
-  (x >>> y) ⦃ z => z.toNat = x.toNat >>> y.toNat ∧ z.toBitVec = x.toBitVec >>> y.toNat ⦄
+  (x >>>? y) ⦃ z => z.toNat = x.toNat >>> y.toNat ∧ z.toBitVec = x.toBitVec >>> y.toNat ⦄
   := by apply UScalar.ShiftRight_IScalar_spec <;> simp [*]
 
 theorem UScalar.ShiftLeft_spec {ty0 ty1} (x : UScalar ty0) (y : UScalar ty1) (size : Nat)
   (hy : y.toNat < ty0.numBits) (hsize : size = UScalar.size ty0) :
-  (x <<< y) ⦃ z =>
+  (x <<<? y) ⦃ z =>
   z.toNat = (x.toNat <<< y.toNat) % size ∧
   z.toBitVec = x.toBitVec <<< y.toNat ⦄
   := by
-  simp only [spec_ok, HShiftLeft.hShiftLeft, shiftLeft_UScalar, shiftLeft, hy, reduceIte, hsize, UScalar.size]
+  simp only [spec_ok, ResultShiftLeft.shiftLeft, shiftLeft_UScalar, shiftLeft, hy, reduceIte, hsize, UScalar.size]
   simp only [BitVec.shiftLeft_eq, toNat]
-  simp only [toBitVec_toNat, BitVec.toNat_shiftLeft, ShiftLeft.shiftLeft, Nat.shiftLeft_eq', and_self]
+  simp only [toBitVec_toNat, BitVec.toNat_shiftLeft, and_self]
 
 uscalar @[step] theorem «%S».ShiftLeft_spec {ty1} (x : «%S») (y : UScalar ty1) (hy : y.toNat < %BitWidth) :
-  (x <<< y) ⦃ z => z.toNat = (x.toNat <<< y.toNat) % «%S».size ∧ z.toBitVec = x.toBitVec <<< y.toNat ⦄
+  (x <<<? y) ⦃ z => z.toNat = (x.toNat <<< y.toNat) % «%S».size ∧ z.toBitVec = x.toBitVec <<< y.toNat ⦄
   := by apply UScalar.ShiftLeft_spec <;> simp [*]
 
 theorem UScalar.ShiftLeft_IScalar_spec {ty0 ty1} (x : UScalar ty0) (y : IScalar ty1) (size : Nat)
-  (hy0 : 0 ≤ y.toNat) (hy1 : y.toNat < ty0.numBits) (hsize : size = UScalar.size ty0) :
-  (x <<< y) ⦃ z =>
+  (_hy0 : 0 ≤ y.toNat) (hy1 : y.toNat < ty0.numBits) (hsize : size = UScalar.size ty0) :
+  (x <<<? y) ⦃ z =>
   z.toNat = (x.toNat <<< y.toNat) % size ∧
   z.toBitVec = x.toBitVec <<< y.toNat ⦄
   := by
   have hy1 : y.toNat < ty0.numBits := by scalar_tac
-  simp only [spec_ok,HShiftLeft.hShiftLeft, shiftLeft_IScalar, shiftLeft, hy1, reduceIte, hsize,
+  simp only [spec_ok, ResultShiftLeft.shiftLeft, shiftLeft_IScalar, shiftLeft, hy1, reduceIte, hsize,
     UScalar.size]
   simp only [BitVec.shiftLeft_eq, toNat]
-  simp only [IScalar.toNat, BitVec.toNat_shiftLeft, toBitVec_toNat, ShiftLeft.shiftLeft,
-    Nat.shiftLeft_eq', and_self]
+  simp only [IScalar.toNat, BitVec.toNat_shiftLeft, toBitVec_toNat, and_self]
 
 uscalar @[step] theorem «%S».ShiftLeft_IScalar_spec {ty1} (x : «%S») (y : IScalar ty1) (hy0 : 0 ≤ y.toNat) (hy : y.toNat < %BitWidth) :
-  (x <<< y) ⦃ z => z.toNat = (x.toNat <<< y.toNat) % «%S».size ∧ z.toBitVec = x.toBitVec <<< y.toNat ⦄
+  (x <<<? y) ⦃ z => z.toNat = (x.toNat <<< y.toNat) % «%S».size ∧ z.toBitVec = x.toBitVec <<< y.toNat ⦄
   := by apply UScalar.ShiftLeft_IScalar_spec <;> simp [*]
 
 /-!
