backends/lean/Aeneas/Std/Scalar/CheckedOps/Rem.lean
@@ -39,7 +39,7 @@ theorem core.num.checked_rem_UScalar_bv_spec {ty} (x y : UScalar ty) :
   . rename_i hnz
     simp
     have hnz' : y.toNat ≠ 0 := by zify at *; simp_all
-    have : x % y = x.rem y := by rfl
+    have : x %? y = x.rem y := by rfl
     have ⟨_, hz⟩ := spec_imp_exists (UScalar.rem_toBitVec_spec x hnz')
     simp [this, UScalar.rem, hnz] at hz
     simp [hz, hnz']
@@ -67,7 +67,7 @@ theorem core.num.checked_rem_IScalar_bv_spec {ty} (x y : IScalar ty) :
   . rename_i hnz
     simp
     have hnz' : y.toInt ≠ 0 := by zify at *; simp_all
-    have : x % y = x.rem y := by rfl
+    have : x %? y = x.rem y := by rfl
     have ⟨ _, hz ⟩ := spec_imp_exists (@IScalar.rem_toBitVec_spec _ x y hnz')
     simp [this, IScalar.rem, hnz] at hz
     simp [*]
