backends/lean/Aeneas/Std/Scalar/CheckedOps/Sub.lean
@@ -11,13 +11,13 @@ open Result Error Arith ScalarElab
 
 /- [core::num::{T}::checked_sub] -/
 def core.num.checked_sub_UScalar {ty} (x y : UScalar ty) : Option (UScalar ty) :=
-  Option.ofResult (x - y)
+  Option.ofResult (x -? y)
 
 uscalar def «%S».checked_sub (x y : «%S») : Option «%S» := core.num.checked_sub_UScalar x y
 
 /- [core::num::{T}::checked_sub] -/
 def core.num.checked_sub_IScalar {ty} (x y : IScalar ty) : Option (IScalar ty) :=
-  Option.ofResult (x - y)
+  Option.ofResult (x -? y)
 
 iscalar def «%S».checked_sub (x y : «%S») : Option «%S» := core.num.checked_sub_IScalar x y
 
@@ -33,7 +33,7 @@ theorem core.num.checked_sub_UScalar_bv_spec {ty} (x y : UScalar ty) :
   | some z => y.toNat ≤ x.toNat ∧ z.toNat = x.toNat - y.toNat ∧ z.toBitVec = x.toBitVec - y.toBitVec
   | none => x.toNat < y.toNat := by
   have h := UScalar.sub_equiv x y
-  have hsub : x - y = UScalar.sub x y := by rfl
+  have hsub : x -? y = UScalar.sub x y := by rfl
   rw [hsub] at h
   cases hEq : UScalar.sub x y <;> simp_all [Option.ofResult, checked_sub_UScalar]
 
@@ -54,7 +54,7 @@ theorem core.num.checked_sub_IScalar_bv_spec {ty} (x y : IScalar ty) :
   | some z => IScalar.min ty ≤ x.toInt - y.toInt ∧ x.toInt - y.toInt ≤ IScalar.max ty ∧ z.toInt = x.toInt - y.toInt ∧ z.toBitVec = x.toBitVec - y.toBitVec
   | none => ¬ (IScalar.min ty ≤ x.toInt - y.toInt ∧ x.toInt - y.toInt ≤ IScalar.max ty) := by
   have h := IScalar.sub_equiv x y
-  have hsub : x - y = IScalar.sub x y := by rfl
+  have hsub : x -? y = IScalar.sub x y := by rfl
   rw [hsub] at h
   cases hEq : IScalar.sub x y <;> simp_all [Option.ofResult, checked_sub_IScalar, IScalar.min, IScalar.max] <;>
   (have : 0 < 2^ty.numBits := by simp) <;>
