backends/lean/Aeneas/Std/Scalar/Ops/Add.lean
@@ -23,25 +23,29 @@ def UScalar.try_add {ty : UScalarTy} (x y : UScalar ty) : Option (UScalar ty) :=
 def IScalar.try_add {ty : IScalarTy} (x y : IScalar ty) : Option (IScalar ty) :=
   Option.ofResult (add x y)
 
-instance {ty} : HAdd (UScalar ty) (UScalar ty) (Result (UScalar ty)) where
-  hAdd x y := UScalar.add x y
+class ResultAdd (α : Type u) where
+  add : α → α → Result α
 
-instance {ty} : HAdd (IScalar ty) (IScalar ty) (Result (IScalar ty)) where
-  hAdd x y := IScalar.add x y
+infixl:65 " +? " => ResultAdd.add
 
+instance {ty} : ResultAdd (UScalar ty) where
+  add x y := UScalar.add x y
+
+instance {ty} : ResultAdd (IScalar ty) where
+  add x y := IScalar.add x y
 
 /-!
 # Addition: Theorems
 -/
 
 theorem UScalar.add_equiv {ty} (x y : UScalar ty) :
-  match x + y with
+  match x +? y with
   | ok z => x.toNat + y.toNat < 2^ty.numBits ∧
     z.toNat = x.toNat + y.toNat ∧
     z.toBitVec = x.toBitVec + y.toBitVec
   | fail _ => ¬ (UScalar.inBounds ty (x.toNat + y.toNat))
   | _ => ⊥ := by
-  have : x + y = add x y := by rfl
+  have : x +? y = add x y := by rfl
   rw [this]
   simp [add]
   have h := tryMk_eq ty (↑x + ↑y)
@@ -53,14 +57,14 @@ theorem UScalar.add_equiv {ty} (x y : UScalar ty) :
   simp [*]
 
 theorem IScalar.add_equiv {ty} (x y : IScalar ty) :
-  match x + y with
+  match x +? y with
   | ok z =>
     IScalar.inBounds ty (x.toInt + y.toInt) ∧
     z.toInt = x.toInt + y.toInt ∧
     z.toBitVec = x.toBitVec + y.toBitVec
   | fail _ => ¬ (IScalar.inBounds ty (x.toInt + y.toInt))
   | _ => ⊥ := by
-  have : x + y = add x y := by rfl
+  have : x +? y = add x y := by rfl
   rw [this]
   simp [add]
   have h := tryMk_eq ty (↑x + ↑y)
@@ -79,7 +83,7 @@ integers and bit-vectors.
 /-- Generic theorem - shouldn't be used much -/
 theorem UScalar.add_toBitVec_spec {ty} {x y : UScalar ty}
   (hmax : ↑x + ↑y ≤ UScalar.max ty) :
-  x + y ⦃ z => (↑z : Nat) = ↑x + ↑y ∧ z.toBitVec = x.toBitVec + y.toBitVec ⦄ := by
+  x +? y ⦃ z => (↑z : Nat) = ↑x + ↑y ∧ z.toBitVec = x.toBitVec + y.toBitVec ⦄ := by
   have h := @add_equiv ty x y
   split at h <;> simp_all [max]
   have : 0 < 2^ty.numBits := by simp
@@ -89,18 +93,18 @@ theorem UScalar.add_toBitVec_spec {ty} {x y : UScalar ty}
 theorem IScalar.add_toBitVec_spec {ty}  {x y : IScalar ty}
   (hmin : IScalar.min ty ≤ ↑x + ↑y)
   (hmax : ↑x + ↑y ≤ IScalar.max ty) :
-  x + y ⦃ z => (↑z : Int) = ↑x + ↑y ∧ z.toBitVec = x.toBitVec + y.toBitVec ⦄ := by
+  x +? y ⦃ z => (↑z : Int) = ↑x + ↑y ∧ z.toBitVec = x.toBitVec + y.toBitVec ⦄ := by
   have h := @add_equiv ty x y
   split at h <;> simp_all [min, max]
   omega
 
 uscalar theorem «%S».add_bv_spec {x y : «%S»} (hmax : x.toNat + y.toNat ≤ «%S».max) :
-  x + y ⦃ z => (↑z : Nat) = ↑x + ↑y ∧ z.toBitVec = x.toBitVec + y.toBitVec ⦄ :=
+  x +? y ⦃ z => (↑z : Nat) = ↑x + ↑y ∧ z.toBitVec = x.toBitVec + y.toBitVec ⦄ :=
   UScalar.add_toBitVec_spec (by scalar_tac)
 
 iscalar theorem «%S».add_bv_spec {x y : «%S»}
   (hmin : «%S».min ≤ ↑x + ↑y) (hmax : ↑x + ↑y ≤ «%S».max) :
-  x + y ⦃ z => (↑z : Int) = ↑x + ↑y ∧ z.toBitVec = x.toBitVec + y.toBitVec ⦄ :=
+  x +? y ⦃ z => (↑z : Int) = ↑x + ↑y ∧ z.toBitVec = x.toBitVec + y.toBitVec ⦄ :=
   IScalar.add_toBitVec_spec (by scalar_tac) (by scalar_tac)
 
 /-!
@@ -113,7 +117,7 @@ only integers. Those are the most common to use, so we mark them with the
 @[step]
 theorem UScalar.add_spec {ty} {x y : UScalar ty}
   (hmax : ↑x + ↑y ≤ UScalar.max ty) :
-  x + y ⦃ z => (↑z : Nat) = ↑x + ↑y ⦄ := by
+  x +? y ⦃ z => (↑z : Nat) = ↑x + ↑y ⦄ := by
   have h := @add_equiv ty x y
   split at h <;> simp_all [max]
   have : 0 < 2^ty.numBits := by simp
@@ -124,18 +128,18 @@ theorem UScalar.add_spec {ty} {x y : UScalar ty}
 theorem IScalar.add_spec {ty} {x y : IScalar ty}
   (hmin : IScalar.min ty ≤ ↑x + ↑y)
   (hmax : ↑x + ↑y ≤ IScalar.max ty) :
-  x + y ⦃ z => (↑z : Int) = ↑x + ↑y ⦄ := by
+  x +? y ⦃ z => (↑z : Int) = ↑x + ↑y ⦄ := by
   have h := @add_equiv ty x y
   split at h <;> simp_all [min, max]
   omega
 
 uscalar @[step] theorem «%S».add_spec {x y : «%S»} (hmax : x.toNat + y.toNat ≤ «%S».max) :
-  x + y ⦃ z => (↑z : Nat) = ↑x + ↑y ⦄ :=
+  x +? y ⦃ z => (↑z : Nat) = ↑x + ↑y ⦄ :=
   UScalar.add_spec (by scalar_tac)
 
 iscalar @[step] theorem «%S».add_spec {x y : «%S»}
   (hmin : «%S».min ≤ ↑x + ↑y) (hmax : ↑x + ↑y ≤ «%S».max) :
-  x + y ⦃ z => (↑z : Int) = ↑x + ↑y ⦄ :=
+  x +? y ⦃ z => (↑z : Int) = ↑x + ↑y ⦄ :=
   IScalar.add_spec (by scalar_tac) (by scalar_tac)
 
 end Aeneas.Std
